theories/Compositional_Structures/Basic_Modules/Component_Types/Social_Choice_Types/Profile_List_Monadic.thy
@@ -901,6 +901,7 @@ sepref_definition limit_sep is "uncurry (limit_profile_l)" ::
   apply (rewrite in "WHILEIT _ _ _ \<hole>" arl.fold_custom_empty)
   by sepref
 
+
 lemma "limitp_correct":
   shows "(limit_profile_l, RETURN oo limit_profile) \<in> 
       \<langle>Id\<rangle>alt_set_rel \<rightarrow> profile_rel \<rightarrow> \<langle>profile_rel\<rangle>nres_rel"
