theories/Compositional_Structures/Elect_Composition_Ref.thy
@@ -1,9 +1,27 @@
 theory Elect_Composition_Ref
   imports "Basic_Modules/Elect_Module_Ref"
+          "Verified_Voting_Rule_Construction.Elect_Composition"
           Sequential_Composition_Ref
 begin
 
-fun elector_ref :: "'a Electoral_Module_Ref \<Rightarrow> 'a Electoral_Module_Ref" where
-  "elector_ref m = (m \<triangleright>r elect_module_ref)"
+
+definition  
+  "elector_sep m \<equiv> m \<triangleright>sep elect_module_sep"
+
+lemma elector_sep_impl: "seqcomp_impl m_ref m_impl elect_module_ref elect_module_sep"
+  apply unfold_locales
+proof -
+  show "(uncurry elect_module_sep, uncurry elect_module_ref)
+    \<in> (hs.assn nat_assn)\<^sup>k *\<^sub>a
+       profile_impl_assn\<^sup>k \<rightarrow>\<^sub>a hs.assn nat_assn \<times>\<^sub>a hs.assn nat_assn \<times>\<^sub>a hs.assn nat_assn"
+    using elect_module_sep.refine by simp
+next
+
+  oops
+
+interpretation electori:  seqcomp_impl m_ref m_impl elect_module_ref elect_module_sep
+
+  oops
+
 
 end
